prove 3DM to X3C Poly ( and refine the algo for JobSeq)

Karp21/SS_To_JS/SS_List_To_Job_Seq_Poly.thy
@@ -4,11 +4,20 @@ theory SS_List_To_Job_Seq_Poly
          SS_To_JS_aux
 begin
 
-section "The reduction from subset sum list to job sequence is polynomial"
+section "costs"
 
+definition size_job_seq where
+  "size_job_seq = (\<lambda> (ps, ds, ws, k).  length ps + length ds + length ws + 1)"
 
-subsection "Algorithm Definition"
+definition ss_list_to_job_seq_time :: "nat \<Rightarrow> nat" where
+  "ss_list_to_job_seq_time n = 2 * n" 
 
+definition ss_list_to_job_seq_space :: "nat \<Rightarrow> nat" where
+  "ss_list_to_job_seq_space n = 3 * n + 1"
+
+section "first refinement"
+
+text \<open>we assume that one can add a list and replicate a value in time of length of the list\<close>
 definition mop_sum_list where
   "mop_sum_list ws \<equiv> SPECT [sum_list ws \<mapsto>  length ws]"
                         
@@ -27,19 +36,8 @@ definition ss_list_to_job_seq_alg :: "(nat list \<times> nat) \<Rightarrow> (nat
       else RETURNT NOT_JOB_SEQ_EXAMPLE
     }"
 
-(* check phd thesis max *)
-subsection "Time and Space Definitions"
-
-definition ss_list_to_job_seq_time :: "nat \<Rightarrow> nat" where
-  "ss_list_to_job_seq_time n = 2*n" 
-
-definition ss_list_to_job_seq_space :: "nat \<Rightarrow> nat" where
-  "ss_list_to_job_seq_space n = 3 * n + 1"
-
-definition size_job_seq where
-  "size_job_seq = (\<lambda> (ps, ds, ws, k).  length ps + length ds + length ws + 1)"
-
 subsection "Proofs"
+
 
 lemma ss_list_to_job_seq_refines:
   "ss_list_to_job_seq_alg P 
@@ -64,6 +62,109 @@ theorem ss_list_to_job_seq_is_polyred:
   by (intro ispolyredI[where ?time_f  = ss_list_to_job_seq_time  and
                              ?space_f = ss_list_to_job_seq_space],
       unfold ss_list_to_job_seq_time_def ss_list_to_job_seq_space_def) fast+
- 
 
+
+section "second refinement"
+
+text \<open>we relax the assumptions to:
+     -  we can add two numbers in constant time 
+     -  we can add a constant to front in constant time\<close>
+
+definition mop_add where
+  "mop_add a b \<equiv> SPECT [a + b \<mapsto> 1]"
+
+definition mop_const_cons where
+  "mop_const_cons c _ xs \<equiv> SPECT [ (c # xs) \<mapsto> 1]"
+
+definition ss_list_to_job_seq_alg2 :: "(nat list \<times> nat) \<Rightarrow> (nat list \<times> nat list \<times> nat list \<times> nat) nrest" where
+  "ss_list_to_job_seq_alg2 \<equiv> \<lambda>(ws, B).
+    do {
+      s \<leftarrow> nfoldli ws (\<lambda>_. True) mop_add 0;
+      if s \<ge> B
+      then do {
+        ds \<leftarrow>  nfoldli ws (\<lambda>_. True) (mop_const_cons B) [];
+        RETURNT (ws, ds, ws, s - B)
+      }
+      else RETURNT NOT_JOB_SEQ_EXAMPLE
+    }"
+
+
+lemma sum_list_linear:
+  "nfoldli (P:: nat list)(\<lambda>_. True) mop_add k 
+   \<le> SPEC (\<lambda>y. y = (sum_list P) + k) (\<lambda>_. length P)"
+proof (induction P arbitrary: k )
+  case Nil
+  then show ?case
+    by (simp add: inresT_SPEC pw_le_iff)
+next
+  case (Cons x xs)
+  have "mop_add x k = SPECT [x + k \<mapsto> 1]"
+    by (simp add:  mop_add_def)
+  moreover have "nfoldli xs (\<lambda>_. True) mop_add (x + k) 
+                 \<le> SPEC (\<lambda>y. y =  sum_list xs + (x + k)) (\<lambda>_. length xs)"
+    using Cons.IH[of "x + k"] by simp
+  ultimately have *: "nfoldli (x # xs) (\<lambda>_. True) mop_add k \<le> do {
+    s1 \<leftarrow> SPECT [x + k \<mapsto> 1];
+    y \<leftarrow> SPEC (\<lambda>y. y =  sum_list xs + s1) (\<lambda>_. length xs);
+    RETURNT y
+  }" 
+    using bindT_mono' Cons by fastforce
+  moreover have "do {
+            s1 \<leftarrow> SPECT [k + x \<mapsto> 1];
+            y \<leftarrow> SPEC (\<lambda>y. y = sum_list xs + s1) (\<lambda>_. length xs );
+            RETURNT y
+          } \<le> SPEC (\<lambda>y. y = sum_list (x#xs) + k) (\<lambda>_. length xs + 1)"
+      unfolding SPEC_def  
+      apply (vcg)
+      unfolding bindT_def 
+      by (auto simp add: add.commute le_fun_def one_enat_def)
+  ultimately show ?case
+    by (simp add: SPEC_def add.commute)
+qed
+
+lemma replicate_linear:
+  "nfoldli P (\<lambda>_. True) (mop_const_cons B) k
+   \<le> SPEC (\<lambda>y. y = (replicate (length P) B)@k) (\<lambda>_. length P)"
+proof (induction P arbitrary: k )
+  case Nil
+  then show ?case
+    by (simp add: inresT_SPEC pw_le_iff)
+next
+  case (Cons x xs)
+  have "mop_const_cons B x k = SPECT [B # k \<mapsto> 1]"
+    by (simp add:  mop_const_cons_def)
+  moreover have "nfoldli xs (\<lambda>_. True) (mop_const_cons B) (B#k)
+                 \<le> SPEC (\<lambda>y. y = (replicate (length xs) B)@(B#k)) (\<lambda>_. length xs)"
+    using Cons.IH[of "B#k"] by simp
+  ultimately have *: "nfoldli (x#xs) (\<lambda>_. True) (mop_const_cons B) k \<le> do {
+    s1 \<leftarrow> SPECT [B # k \<mapsto> 1];
+    y \<leftarrow> SPEC (\<lambda>y. y = (replicate (length xs) B)@s1) (\<lambda>_. length xs);
+    RETURNT y
+  }"   
+    using bindT_mono' Cons 
+    by fastforce
+  moreover have "do {
+            s1 \<leftarrow> SPECT [B # k \<mapsto> 1];
+            y \<leftarrow> SPEC (\<lambda>y. y = (replicate (length xs) B)@s1) (\<lambda>_. length xs);
+            RETURNT y
+          } \<le> SPEC (\<lambda>y. y = (replicate (length (x#xs)) B)@k) (\<lambda>_. length xs + 1)"
+      unfolding SPEC_def  
+      apply (vcg)
+      unfolding bindT_def 
+      by (simp add: le_fun_def one_enat_def replicate_app_Cons_same)
+    ultimately show ?case
+      by (simp add: SPEC_def)
+qed
+
+lemma ss_list_to_job_seq_alg2_refines:
+  "ss_list_to_job_seq_alg2 P 
+   \<le> ss_list_to_job_seq_alg P "
+  unfolding ss_list_to_job_seq_alg2_def 
+            ss_list_to_job_seq_alg_def SPEC_def 
+            mop_sum_list_def mop_replicate_B_def
+  apply (refine_mono)
+  by (auto intro!: sum_list_linear[where ?k =0, simplified, THEN ord_le_eq_trans]
+                   replicate_linear[where ?k ="[]", simplified, THEN ord_le_eq_trans]
+           simp add:SPEC_def fun_upd_def)
+ 
 end
